GradVer20Hook.v
@@ -1,7 +1,31 @@
 Load GradVer19Theorems.
 Import Semantics.
 
+Definition phiEquals (p1 p2 : phi) :=
+  forall H r A, evalphi H r A p1 <-> evalphi H r A p2.
 
+Definition wrapHoare (hoare : phi -> s -> phi -> Prop) p1 s p2 : Prop :=
+  exists p1x p2x,
+  phiImplies p1x p1 /\
+  phiImplies p2 p2x /\
+  hoare p1 s p2.
+
+Theorem hoareMiniEquals : forall p1 p2 s,
+  wrapHoare hoareSinglePreMini p1 s p2 <->
+  wrapHoare hoareSingle        p1 s p2.
+Proof.
+  unfold wrapHoare. split; intros; unf.
+  - rename H1 into im1.
+    rename H0 into im2.
+    rename H3 into ho.
+    admit.
+  - rename H1 into im1.
+    rename H0 into im2.
+    rename H3 into ho.
+    admit.
+Admitted.
+
+(* 
 Definition dfrme H r (A : A_d) (e : e) := 
   evale' H r e <> None /\ incl (footprintXe H r e) A.
 
@@ -37,4 +61,4 @@ Proof.
   - eex.
   - split; auto.
     discriminate.
-Qed.
+Qed. *)
